common/Events.v
@@ -1964,3 +1964,151 @@ Qed.
 
 End EVAL_BUILTIN_ARG_LESSDEF.
 
+Section INFORM_TRACES.
+
+Variable F V: Type.
+Variable ge: Genv.t F V.
+
+Inductive call_trace: compartment -> compartment -> val -> list val -> list typ -> trace -> Prop :=
+  | call_trace_intra: forall cp cp' vf vargs ty,
+    Genv.type_of_call ge cp cp' <> Genv.CrossCompartmentCall ->
+    call_trace cp cp' vf vargs ty E0
+  | call_trace_cross: forall cp cp' vf vargs vl ty b ofs i,
+      Genv.type_of_call ge cp cp' = Genv.CrossCompartmentCall ->
+      vf = Vptr b ofs ->
+      Genv.invert_symbol ge b = Some i ->
+      eventval_list_match ge vl ty vargs ->
+      call_trace cp cp' vf vargs ty (Event_call cp cp' i vl :: nil).
+
+Lemma call_trace_same_cp:
+  forall cp vf vargs tyargs t,
+    call_trace cp cp vf vargs tyargs t ->
+    t = E0.
+Proof.
+  intros. inv H; auto.
+  now apply Genv.type_of_call_same_cp in H0.
+Qed.
+
+Inductive return_trace: compartment -> compartment -> val -> rettype -> trace -> Prop :=
+| return_trace_intra: forall cp cp' v ty,
+    Genv.type_of_call ge cp cp' <> Genv.CrossCompartmentCall ->
+    return_trace cp cp' v ty E0
+| return_trace_cross: forall cp cp' res v ty,
+    Genv.type_of_call ge cp cp' = Genv.CrossCompartmentCall ->
+    eventval_match ge res (proj_rettype ty) v ->
+    return_trace cp cp' v ty (Event_return cp cp' res :: nil)
+.
+
+End INFORM_TRACES.
+
+Section INFORM_TRACES_INJECT.
+  Variable F V: Type.
+  Variable F' V': Type.
+  Variable ge: Genv.t F V.
+  Variable ge': Genv.t F' V'.
+
+  Variable j: meminj.
+
+  (* I couldn't find a way to prove that with using [symbols_preserved]. *)
+  Lemma call_trace_inj (symbols_preserved: forall (s: ident), Genv.find_symbol ge' s = Genv.find_symbol ge s):
+    forall cp cp' vf vs vs' tys t,
+      Val.inject_list j vs vs' ->
+      (Genv.type_of_call ge cp cp' = Genv.CrossCompartmentCall -> Forall not_ptr vs) ->
+      call_trace ge cp cp' vf vs tys t ->
+      call_trace ge' cp cp' vf vs' tys t.
+  Proof.
+    intros cp cp' vf vs vs' tys t LD NPTR EV.
+    inv EV.
+    - constructor; auto.
+    - specialize (NPTR H).
+      econstructor; eauto. apply Genv.find_invert_symbol.
+      rewrite symbols_preserved.
+      eapply Genv.invert_find_symbol; eauto.
+      clear -LD NPTR H2.
+      revert vs vs' tys vl LD NPTR H2.
+      induction vs; intros vs' tys vl LD NPTR Hmatch.
+      + inv LD; inv Hmatch; constructor.
+      + inv LD; inv Hmatch; inv NPTR.
+        constructor; eauto.
+        inv H1; inv H5; try contradiction; econstructor; eauto.
+  Qed.
+
+  Lemma return_trace_inj:
+    forall cp cp' v v' ty t,
+      Val.inject j v v' ->
+      (Genv.type_of_call ge cp cp' = Genv.CrossCompartmentCall -> not_ptr v) ->
+      return_trace ge cp cp' v ty t ->
+      return_trace ge' cp cp' v' ty t.
+  Proof.
+    intros cp cp' v v' ty t LD NPTR EV.
+    inv EV.
+    - constructor; auto.
+    - constructor; auto.
+      specialize (NPTR H).
+      inv LD; inv H0; try econstructor; eauto.
+      inv NPTR.
+  Qed.
+
+End INFORM_TRACES_INJECT.
+
+Section INFORM_TRACES_PRESERVED.
+  Variable F V: Type.
+  Variable F' V': Type.
+  Variable ge: Genv.t F V.
+  Variable ge': Genv.t F' V'.
+
+  Variable symbols_preserved: forall (s: ident), Genv.find_symbol ge' s = Genv.find_symbol ge s.
+  Variable senv_preserved: Senv.equiv ge ge'.
+
+  Lemma call_trace_lessdef:
+    forall cp cp' vf vs vs' tys t,
+      Val.lessdef_list vs vs' ->
+      call_trace ge cp cp' vf vs tys t ->
+      call_trace ge' cp cp' vf vs' tys t.
+  Proof.
+    intros cp cp' vf vs vs' tys t LD EV.
+    inv EV.
+    - constructor; auto.
+    - econstructor; eauto.
+      apply Genv.invert_find_symbol in H1.
+      apply Genv.find_invert_symbol.
+      now rewrite symbols_preserved.
+      eapply eventval_list_match_lessdef; eauto.
+      eapply eventval_list_match_preserved with (ge1 := ge); try eapply senv_preserved; eauto.
+  Qed.
+
+  Lemma call_trace_eq:
+    forall cp cp' vf vs tys t,
+      call_trace ge cp cp' vf vs tys t ->
+      call_trace ge' cp cp' vf vs tys t.
+    Proof.
+      intros.
+      eapply call_trace_lessdef; eauto.
+      clear.
+      induction vs; eauto.
+    Qed.
+
+  Lemma return_trace_lessdef:
+    forall cp cp' v v' ty t,
+      Val.lessdef v v' ->
+      return_trace ge cp cp' v ty t ->
+      return_trace ge' cp cp' v' ty t.
+  Proof.
+    intros cp cp' v v' ty t LD EV.
+    inv EV.
+    - constructor; auto.
+    - constructor; auto.
+      eapply eventval_match_lessdef; eauto.
+      eapply eventval_match_preserved with (ge1 := ge); try eapply senv_preserved; eauto.
+  Qed.
+
+  Lemma return_trace_eq:
+    forall cp cp' v ty t,
+      return_trace ge cp cp' v ty t ->
+      return_trace ge' cp cp' v ty t.
+  Proof.
+    intros.
+    eapply return_trace_lessdef; eauto using Val.lessdef_refl.
+  Qed.
+
+End INFORM_TRACES_PRESERVED.
